src/SDK/Client.dfy
@@ -68,8 +68,8 @@ module ESDKClient {
     var unauthenticatedHeader := wr.data;
 
     var iv: seq<uint8> := seq(encMat.algorithmSuiteID.IVLength(), _ => 0);
-    var authenticationTag :- AuthTag(encMat.algorithmSuiteID, iv, derivedDataKey, unauthenticatedHeader);
-    var headerAuthentication := Msg.HeaderAuthentication(iv, authenticationTag);
+    var encryptionOutput :- AESEncryption.AESEncrypt(encMat.algorithmSuiteID.Algorithm(), iv, derivedDataKey, [], unauthenticatedHeader);
+    var headerAuthentication := Msg.HeaderAuthentication(iv, encryptionOutput.authTag);
     var _ :- Serialize.SerializeHeaderAuthentication(wr, headerAuthentication, encMat.algorithmSuiteID);
 
     /*
@@ -116,18 +116,5 @@ module ESDKClient {
     var len := algorithmSuiteID.KeyLength();
     var derivedKey := HKDF.hkdf(whichSHA, None, inputKeyMaterials, info, len);
     return derivedKey[..];
-  }
-
-  method AuthTag(algorithmSuiteID: AlgorithmSuite.ID, iv: seq<uint8>, key: seq<uint8>, aad: seq<uint8>) returns (res: Result<seq<uint8>>)
-    requires |iv| == algorithmSuiteID.IVLength()
-    requires |key| == algorithmSuiteID.KeyLength()
-    ensures match res
-      case Success(authTag) =>
-        |authTag| == algorithmSuiteID.TagLength()
-      case Failure(_) => true
-  {
-    var cipher := AlgorithmSuite.Suite[algorithmSuiteID].algorithm;
-    var encryptionOutput :- AESEncryption.AESEncrypt(cipher, iv, key, [], aad);
-    return Success(encryptionOutput.authTag);
   }
 }
